Re-implements the switcher (and the macros it uses) with Griotte assembler

theories/switcher/clear_stack.v
@@ -1,134 +1,32 @@
-From iris.algebra Require Import frac.
-From iris.proofmode Require Import proofmode.
-From cap_machine Require Import memory_region rules proofmode.
+From cap_machine Require Import machine_parameters assembler.
 
 Section ClearStackMacro.
-  Context
-    {Σ:gFunctors}
-    {ceriseg:ceriseG Σ}
-    `{MP: MachineParameters}.
+  Import Asm_Griotte.
+  Local Coercion Z.of_nat : nat >-> Z.
+  Context `{MP: MachineParameters}.
 
   (* Expects r1 := e_stk ; r2 := a_stk *)
+  Definition clear_stack_asm_pre (r1 r2 : RegName) : list asm_code :=
+    [
+      sub r1 r2 r1;
+      mov r2 csp;
+      #"loop_start";
+      jnz ("loop_body")%asm r1;
+      jmp ("loop_end")%asm;
+      #"loop_body";
+      store r2 0;
+      lea r2 1;
+      add r1 r1 1;
+      jmp ("loop_start")%asm;
+      #"loop_end"
+    ].
+
+  Definition clear_stack_asm_env :=
+    Eval vm_compute in (compute_asm_code_env (clear_stack_asm_pre PC PC)).2.
+  Definition clear_stack_asm (r1 r2 : RegName) :=
+    Eval compute in resolve_labels_macros (clear_stack_asm_pre r1 r2) clear_stack_asm_env.
+  Definition clear_stack (r1 r2 : RegName) : list instr :=
+    Eval compute in assemble (clear_stack_asm r1 r2).
   Definition clear_stack_instrs (r1 r2 : RegName) : list Word :=
-    encodeInstrsW [
-        Sub r1 r2 r1;
-        Mov r2 csp;
-        Jnz 2%Z r1;
-        Jmp 5%Z;
-        Store r2 0%Z;
-        Lea r2 1%Z;
-        Add r1 r1 1%Z;
-        Jmp (-5)%Z
-      ].
-
-  Lemma clear_stack_spec
-    (pc_p : Perm) (pc_g : Locality) (pc_b pc_e pc_a : Addr)
-    (csp_g : Locality) (csp_b csp_e csp_a : Addr)
-    (r1 r2 : RegName) (ws : list Word)
-    φ :
-    executeAllowed pc_p = true ->
-    SubBounds pc_b pc_e pc_a (pc_a ^+ length (clear_stack_instrs r1 r2))%a ->
-    (csp_b <= csp_a)%a -> (csp_a <= csp_e)%a ->
-    ( PC ↦ᵣ WCap pc_p pc_g pc_b pc_e pc_a
-      ∗ csp ↦ᵣ WCap RWL csp_g csp_b csp_e csp_a
-      ∗ r1 ↦ᵣ WInt csp_e ∗ r2 ↦ᵣ WInt csp_a
-      ∗ codefrag pc_a (clear_stack_instrs r1 r2)
-      ∗ ([[ csp_a , csp_e ]] ↦ₐ [[ ws ]])
-      ∗ ▷ ( (PC ↦ᵣ WCap pc_p pc_g pc_b pc_e (pc_a ^+ length (clear_stack_instrs r1 r2))%a
-             ∗ csp ↦ᵣ WCap RWL csp_g csp_b csp_e csp_a
-             ∗ r1 ↦ᵣ WInt 0 ∗ r2 ↦ᵣ WCap RWL csp_g csp_b csp_e csp_e
-             ∗ codefrag pc_a (clear_stack_instrs r1 r2)
-             ∗ ([[ csp_a , csp_e ]] ↦ₐ [[region_addrs_zeroes csp_a csp_e]]))
-        -∗ WP Seq (Instr Executable) {{ φ }})
-      ∗ ▷ φ FailedV
-    )
-      ⊢ WP Seq (Instr Executable) {{ φ }}%I.
-  Proof.
-    iIntros (Hpc_exec Hbounds Hbounds1 Hbounds2)
-      "(HPC & Hcsp & Hr1 & Hr2 & Hcode & Hstack & Hφ & Hfail)".
-    codefrag_facts "Hcode".
-
-    (* --- Sub r1 r2 r1 --- *)
-    iInstr "Hcode".
-
-    (* --- Mov r2 csp --- *)
-    iInstr "Hcode".
-
-    remember (WCap RWL csp_g csp_b csp_e csp_a) as sp.
-    rewrite{2} Heqsp. clear Heqsp.
-    iAssert (⌜(csp_b <= csp_a)%a ⌝)%I as "-#Hbounds1"; first done.
-    iAssert (⌜(csp_a <= csp_e)%a ⌝)%I as "-#Hbounds2"; first done.
-    clear Hbounds1 Hbounds2.
-    iLöb as "IH" forall (csp_a ws).
-    iDestruct "Hbounds1" as "%Hbounds1".
-    iDestruct "Hbounds2" as "%Hbounds2".
-    iDestruct (big_sepL2_length with "Hstack") as "%Hlen_stk".
-
-    destruct (decide (csp_a = csp_e)).
-    - (* csp_a = csp_2 ==> loop has ended *)
-      replace (csp_a - csp_e)%Z with 0%Z by solve_addr.
-      (* --- Jnz 2 r1 --- *)
-      iInstr "Hcode".
-      (* --- Jmp 5 ---- *)
-      iInstr "Hcode".
-      iApply "Hφ". subst. iFrame.
-      rewrite /region_pointsto finz_seq_between_empty; last solve_addr+.
-      rewrite /region_addrs_zeroes finz_dist_0; last solve_addr+.
-      done.
-    - (* csp_a ≠ csp_2 ==> another iteration (or failure) *)
-      (* --- Jnz 2 r1 --- *)
-      iInstr_lookup "Hcode" as "Hi" "Hcode".
-      wp_instr.
-      iApply (wp_jnz_success_jmp_z with "[$HPC $Hi $Hr1]"); try solve_pure.
-      { intros Hcontr; inversion Hcontr; solve_addr. }
-      iIntros "!> (HPC & Hi & Hct2)".
-      wp_pure.
-      iSpecialize ("Hcode" with "[$]").
-
-      (* --- Store r2 0%Z --- *)
-      iInstr_lookup "Hcode" as "Hi" "Hcode".
-      wp_instr.
-      rewrite finz_seq_between_cons in Hlen_stk; last solve_addr.
-      destruct ws as [|wa ws]; simplify_eq.
-      rewrite (region_pointsto_cons _ (csp_a ^+ 1)%a); [| solve_addr | solve_addr].
-      iDestruct "Hstack" as "[Ha Hstack]".
-      iApply (wp_store_success_z with "[$HPC $Hi $Hr2 $Ha]"); try solve_pure.
-      { apply withinBounds_true_iff; solve_addr. }
-      iIntros "!> (HPC & Hi & Hr2 & Ha)".
-      wp_pure.
-      iSpecialize ("Hcode" with "[$]").
-
-      (* --- Lea r2 1 --- *)
-      destruct (csp_a + 1)%a eqn:Ha;cycle 1.
-      { iInstr_lookup "Hcode" as "Hi" "Hcode".
-        wp_instr.
-        iApply (wp_Lea_fail_none_z with "[$HPC $Hi $Hr2]")
-        ; try solve_pure
-        ; eauto.
-        iIntros "!> _". wp_pure. wp_end. iFrame. }
-      iInstr "Hcode".
-
-      (* --- Add r1 r1 1 --- *)
-      iInstr "Hcode".
-
-      (* --- Jmp -5 --- *)
-      iInstr "Hcode".
-      { instantiate (1:=(pc_a ^+ 2)%a). solve_addr. }
-
-      (* IH *)
-      replace (csp_a - csp_e + 1)%Z with (f - csp_e)%Z by solve_addr.
-      replace f with (csp_a ^+1)%a by solve_addr.
-      iApply ("IH" $! (csp_a ^+1)%a ws with
-               "[$Hstack] [Ha Hφ] [$Hfail] [$Hct2] [$Hcode] [$HPC] [$Hr2] [$Hcsp] [] []").
-      { iIntros "(?&?&?&?&?&Hstk)".
-        iApply "Hφ"; iFrame.
-        iDestruct ( region_pointsto_cons with "[$Ha $Hstk]" ) as "Hstk"; [solve_addr|solve_addr|].
-        rewrite /region_addrs_zeroes.
-        rewrite (finz_dist_S csp_a); last solve_addr.
-        by cbn.
-      }
-      { iPureIntro ; solve_addr. }
-      { iPureIntro ; solve_addr. }
-  Qed.
-
+    encodeInstrsW (clear_stack r1 r2).
 End ClearStackMacro.
